more progress

LJm/FragmentLambda.v
@@ -9,26 +9,37 @@ Module L := LJm.Definitions.
 
 Import L.LJmNotations.
 
-Inductive is_lambda_tm : term -> Set :=
-| il_var_b (n:nat) : is_lambda_tm (var_b n)
-| il_var_f (x:var) : is_lambda_tm (var_f x)
-| il_abs (t:term) : is_lambda_tm t -> is_lambda_tm (abs t)
+Inductive is_lambda : term -> Prop :=
+| il_var_b (n:nat) : is_lambda (var_b n)
+| il_var_f (x:var) : is_lambda (var_f x)
+| il_abs (t:term) : is_lambda t -> is_lambda (abs t)
 | il_app (t u:term) :
-    is_lambda_tm t ->
-    is_lambda_tm u ->
-    is_lambda_tm (app t (args u anil (cabs (var_b 0)))).
+    is_lambda t ->
+    is_lambda u ->
+    is_lambda (app t (args u anil (cabs (var_b 0)))).
 
-Hint Constructors is_lambda_tm.
+Hint Constructors is_lambda.
 
 Theorem subst_preserves_il u x t :
-  is_lambda_tm u ->
-  is_lambda_tm t ->
-  is_lambda_tm (substT u x t).
+  is_lambda u ->
+  is_lambda t ->
+  is_lambda (substT u x t).
 Proof.
   intros.
   induction H0; simpl; auto.
-  case (x0 == x); auto.
+  - case (x0 == x); auto.
 Qed.
+
+Theorem open_preserves_il u t :
+  is_lambda u ->
+  is_lambda t ->
+  is_lambda (openT u t).
+Admitted.
+
+Lemma beta_preserves_il t1 t2 : is_lambda t1 -> betaT t1 t2 -> is_lambda t2.
+  intros.
+  induction H0.
+  - induction H0. apply open_preserves_il; trivial.
 
 (* Relationship with the external STLC *)
 
@@ -40,27 +51,28 @@ Fixpoint exp_to_terms (e:exp) : term :=
   | S.app t u => app (exp_to_terms t) (args (exp_to_terms u) anil (cabs (var_b 0)))
   end.
 
-Fixpoint terms_to_exp (t:term) (H: is_lambda_tm t) : exp :=
-  match H with
-  | il_var_b n => S.var_b n
-  | il_var_f x => S.var_f x
-  | il_abs t H => S.abs (terms_to_exp t H)
-  | il_app t u H1 H2 => S.app (terms_to_exp t H1) (terms_to_exp u H2)
-  end.
+(* Fixpoint terms_to_exp (t:term) (H: is_lambda t) : exp := *)
+(*   match H with *)
+(*   | il_var_b n => S.var_b n *)
+(*   | il_var_f x => S.var_f x *)
+(*   | il_abs t H => S.abs (terms_to_exp t H) *)
+(*   | il_app t u H1 H2 => S.app (terms_to_exp t H1) (terms_to_exp u H2) *)
+(*   end. *)
 
-Lemma terms_to_exp_id_l t (H: is_lambda_tm t) : exp_to_terms (terms_to_exp t H) = t.
-  induction H; simpl; auto.
-  - rewrite IHis_lambda_tm; trivial.
-  - rewrite IHis_lambda_tm1, IHis_lambda_tm2. trivial.
-Qed.
+(* Lemma terms_to_exp_id_l t (H: is_lambda t) : exp_to_terms (terms_to_exp t H) = t. *)
+(*   induction H; simpl; auto. *)
+(*   - rewrite IHis_lambda; trivial. *)
+(*   - rewrite IHis_lambda1, IHis_lambda2. trivial. *)
+(* Qed. *)
 
-Lemma il_exp_to_terms e : is_lambda_tm (exp_to_terms e).
-  induction e; simpl; auto.
-Defined.
+(* Lemma il_exp_to_terms e : is_lambda (exp_to_terms e). *)
+(*   induction e; simpl; auto. *)
+(* Defined. *)
 
-Lemma exp_to_terms_id_r e : terms_to_exp (exp_to_terms e) (il_exp_to_terms e) = e.
-  induction e; simpl; auto.
-  - rewrite IHe; trivial.
-  - rewrite IHe1, IHe2; trivial.
-Qed.
+(* Print il_exp_to_terms. *)
 
+(* Lemma exp_to_terms_id_r e : terms_to_exp (exp_to_terms e) (il_exp_to_terms e) = e. *)
+(*   induction e; simpl; auto. *)
+(*   - rewrite IHe. trivial. *)
+(*   - rewrite IHe1, IHe2; trivial. *)
+(* Qed. *)
